logics/merge.dfy
@@ -2,138 +2,147 @@ include "Setups.dfy"
 /**********
 (4) merge()
 ***********/
-// merge() merges the neighboring 2 tiles with same value, should satisfy spec 1, 2, 5
+// merge() merges the neighboring 2 tiles with same value, should satisfy spec 1, 2, 3, 5, 6
 // After merging 2 tiles, the number of non-zero tiles should -1
 module Merge {
     import opened Setups
-// We then have a function merge_pair to do the merging given two tiles in a row
-// The merging should satisfy spec 1: only merge tiles with same value
-// the first tile value should be 2 * original value; second tile value shoud be 0
-// Other tiles should not be changed 
-function merge_pair(row: seq<int>, j: int): (res: seq<int>)
-    requires 0 <= j < |row| - 1
-    // spec 1: only merge tiles with the same value
-    requires row[j] == row[j + 1] && row[j] != 0
-    requires IsPowerOfTwo(row[j])
+    // We then have a function merge_pair to do the merging given two tiles in a row
+    // The merging should satisfy spec 1: only merge tiles with same value
+    // the first tile value should be 2 * original value; second tile value shoud be 0
+    // Other tiles should not be changed 
+    function merge_pair(row: seq<int>, j: int): (res: seq<int>)
+        requires 0 <= j < |row| - 1
+        // spec 1: only merge tiles with the same value
+        requires row[j] == row[j + 1] && row[j] != 0
+        requires IsPowerOfTwo(row[j])
 
-    ensures |res| == |row|
-    ensures res[j] == row[j] * 2   // spec 1: after merging, the first tile should be exactly double the original value;
-    ensures res[j+1] == 0    // spec 1: the second tile must be 0
-    ensures IsPowerOfTwo(res[j])    // spec 2: valid value
-    ensures forall k :: 0 <= k < |row| && k != j && k != j + 1 ==> res[k] == row[k]    // does not change other tiles
-    ensures res[j] == 2048 ==> row[j] == 1024     // the generation of winning tile
-    ensures res != row
-    ensures CountNonZerosRow(merge_pair(row, j)) == CountNonZerosRow(row) - 1
-{
-    var r1 := row[j := row[j] * 2];
-    var r2 := r1[j+1 := 0];
-    
-    // proof for CountNonZerosRow(merge_pair(row, j)) == CountNonZerosRow(row) - 1
-    assert CountNonZerosRow(r2) == CountNonZerosRow(row) - 1 by {
-        CountUpdate(row, j, row[j] * 2); 
-        CountUpdate(r1, j+1, 0);
-    }
-    
-    r2 
-}
-
-// We also have a function to record hwo many merges happen to one tile
-// The function is used for the check of spec 1: every tile should only be merged once in one operation
-function update_count(counts: seq<int>, j: int): seq<int>
-    requires 0 <= j < |counts| - 1
-{
-    counts[j := counts[j] + 1][j + 1 := counts[j+1] + 1]
-}
-
-// The merge method should satisfy spec 1, 2, 5
-method merge(grid: Grid) returns (res: Grid, done: bool)
-    requires ValidGrid(grid)
-    requires ValidValues(grid)
-    // precondition for game state
-    requires !HasWinTile(grid)
-    requires !IsLose(grid)
-    // precondition for wellperformed:
-    requires WellPerformedGrid(grid)
-
-    ensures ValidGrid(res)     // spec 5
-    ensures ValidValues(res)     // spec 2
-    ensures !done ==> res == grid   
-    ensures done == (res != grid)
-    ensures !done ==> CountNonZerosGrid(res) == CountNonZerosGrid(grid)
-    ensures done ==> CountNonZerosGrid(res) < CountNonZerosGrid(grid)
-    // spec 1: once merged, will have empty tile and game state cannot be lose
-    ensures done ==> HasEmptyTile(res)
-    ensures !IsLose(res)
-    // for performance
-    ensures !done ==> WellPerformedGrid(res)
-{
-    res := grid;
-    done := false;
-    
-    var i := 0;
-    while i < N
-        invariant 0 <= i <= N
-        invariant ValidGrid(res)
-        invariant ValidValues(res)
-        invariant !done ==> res == grid
-        invariant done <==> res != grid
-        invariant forall k :: i <= k < N ==> res[k] == grid[k]  //current row and later rows remain unsolved
-        invariant done ==> HasEmptyTile(res)
-        invariant !IsLose(res)
-        invariant done ==> CountNonZerosGrid(res) < CountNonZerosGrid(grid)
-        invariant !done ==> CountNonZerosGrid(res) == CountNonZerosGrid(grid)
+        ensures |res| == |row|
+        ensures res[j] == row[j] * 2   // spec 1: after merging, the first tile should be exactly double the original value;
+        ensures res[j+1] == 0    // spec 1: the second tile must be 0
+        ensures IsPowerOfTwo(res[j])    // spec 2: valid value
+        ensures forall k :: 0 <= k < |row| && k != j && k != j + 1 ==> res[k] == row[k]    // does not change other tiles
+        ensures res[j] == 2048 ==> row[j] == 1024     // the generation of winning tile
+        ensures res != row
+        ensures CountNonZerosRow(merge_pair(row, j)) == CountNonZerosRow(row) - 1
     {
-        var j := 0;   // reset j
-        var merged_counts := seq(N, _ => 0);   // initialize the merge count for current row
+        var r1 := row[j := row[j] * 2];
+        var r2 := r1[j+1 := 0];
+        
+        // proof for CountNonZerosRow(merge_pair(row, j)) == CountNonZerosRow(row) - 1
+        assert CountNonZerosRow(r2) == CountNonZerosRow(row) - 1 by {
+            CountUpdate(row, j, row[j] * 2); 
+            CountUpdate(r1, j+1, 0);
+        }
+        
+        r2 
+    }
 
-        while j < N - 1
-            invariant 0 <= j <= N
+    // We also have a function to record hwo many merges happen to one tile
+    // The function is used for the check of spec 1: every tile should only be merged once in one operation
+    function update_count(counts: seq<int>, j: int): seq<int>
+        requires 0 <= j < |counts| - 1
+    {
+        counts[j := counts[j] + 1][j + 1 := counts[j+1] + 1]
+    }
+
+    // The merge method should satisfy spec 1, 2, 3, 5, 6
+    method merge(grid: Grid) returns (res: Grid, done: bool)
+        // Preconditions:
+        // 1. spec 2 & 5: value and grid validity
+        requires ValidGrid(grid)
+        requires ValidValues(grid)
+        // 2. game state
+        requires !HasWinTile(grid)
+        requires !IsLose(grid)
+        // 3. only receives wellperformed grid (after move)
+        requires WellPerformedGrid(grid)
+
+        // Postconditions:
+        // 1. spec 2 & 5: value and grid validity
+        ensures ValidGrid(res)
+        ensures ValidValues(res)
+        // 2. spec 6: if done = true, then the board changes (including count)
+        ensures !done ==> res == grid   
+        ensures done == (res != grid)
+        ensures !done ==> CountNonZerosGrid(res) == CountNonZerosGrid(grid)
+        ensures done ==> CountNonZerosGrid(res) < CountNonZerosGrid(grid)
+        // 3. spec 1 & 3: once merged, will have empty tile and game state cannot be lose
+        ensures done ==> HasEmptyTile(res)
+        ensures !IsLose(res)
+        // 4. spec 6: for performance, if done, can be well-performed or not well-performed; if !done, must be well-performed
+        ensures !done ==> WellPerformedGrid(res)
+    {
+        res := grid;
+        done := false;
+        
+        var i := 0;
+        while i < N
+            invariant 0 <= i <= N
             invariant ValidGrid(res)
             invariant ValidValues(res)
             invariant !done ==> res == grid
-            invariant !done ==> res[i] == grid[i]
             invariant done <==> res != grid
-            invariant |merged_counts| == N
-            invariant forall k :: 0 <= k < N ==> 0 <= merged_counts[k] <= 1
-            invariant forall k :: j <= k < N ==> merged_counts[k] == 0
-            invariant forall k :: i < k < N ==> res[k] == grid[k]   // later rows remain unsolved
-            invariant forall k :: 0 <= k < N && k != i ==> res[k] == (if k < i then res[k] else grid[k])
+            invariant forall k :: i <= k < N ==> res[k] == grid[k]  //current row and later rows remain unsolved
             invariant done ==> HasEmptyTile(res)
             invariant !IsLose(res)
             invariant done ==> CountNonZerosGrid(res) < CountNonZerosGrid(grid)
             invariant !done ==> CountNonZerosGrid(res) == CountNonZerosGrid(grid)
         {
-            if res[i][j] == res[i][j+1] && res[i][j] != 0 
+            var j := 0;   // reset j
+            var merged_counts := seq(N, _ => 0);   // initialize the merge count for current row
+
+            while j < N - 1
+                invariant 0 <= j <= N
+                invariant ValidGrid(res)
+                invariant ValidValues(res)
+                invariant !done ==> res == grid
+                invariant !done ==> res[i] == grid[i]
+                invariant done <==> res != grid
+                invariant |merged_counts| == N
+                // spec 1: for each tile, merge only happens once
+                invariant forall k :: 0 <= k < N ==> 0 <= merged_counts[k] <= 1
+                invariant forall k :: j <= k < N ==> merged_counts[k] == 0
+                invariant forall k :: i < k < N ==> res[k] == grid[k]   // later rows remain unsolved
+                invariant forall k :: 0 <= k < N && k != i ==> res[k] == (if k < i then res[k] else grid[k])
+                invariant done ==> HasEmptyTile(res)
+                invariant !IsLose(res)
+                invariant done ==> CountNonZerosGrid(res) < CountNonZerosGrid(grid)
+                invariant !done ==> CountNonZerosGrid(res) == CountNonZerosGrid(grid)
             {
-                // record before merge
-                var count_before := CountNonZerosGrid(res);
-                var val_before_merge := res[i][j+1]; 
-                var old_res := res; 
-                if !done { assert res[i] == grid[i]; }
+                if res[i][j] == res[i][j+1] && res[i][j] != 0 && merged_counts[j] == 0 && merged_counts[j+1] == 0
+                {
+                    // record before merge
+                    var count_before := CountNonZerosGrid(res);
+                    var val_before_merge := res[i][j+1]; 
+                    var old_res := res; 
+                    if !done { assert res[i] == grid[i]; }
 
-                // merge the same pair
-                var updatedRow := merge_pair(res[i], j);
-                
-                // update the grid
-                res := res[i := updatedRow];
+                    // merge the same pair
+                    var updatedRow := merge_pair(res[i], j);
+                    
+                    // update the grid
+                    res := res[i := updatedRow];
 
-                // show changes in grid
-                GridCountUpdate(old_res, i, updatedRow);
-                assert CountNonZerosGrid(res) == count_before - 1;
-                // proof for !IsLose
-                assert res[i][j+1] == 0;
-                ImpliesNotLose(res);
+                    // show changes in grid
+                    GridCountUpdate(old_res, i, updatedRow);
+                    assert CountNonZerosGrid(res) == count_before - 1;
+                    // proof for !IsLose
+                    assert res[i][j+1] == 0;
+                    ImpliesNotLose(res);
 
-                done := true; 
-                j := j + 2;   // skip the next merged grid
+                    assert 0 <= j < N - 1;
+                    merged_counts := update_count(merged_counts, j);
+                    
+                    done := true; 
+                    j := j + 2;   // skip the next merged grid
+                }
+                else { j := j + 1; }
             }
-            else { j := j + 1; }
+            i := i + 1;
         }
-        i := i + 1;
+        if !done {
+            assert res == grid;
+            assert WellPerformedGrid(res);
+        }
     }
-    if !done {
-        assert res == grid;
-        assert WellPerformedGrid(res);
-    }
-}
 }
